Examples/EdmondsKarp_Maxflow/Augmenting_Path_BFS_Impl.thy
@@ -9,19 +9,35 @@ begin
 subsection \<open>Imperative Implementation\<close>
 
 term Augmenting_Path_BFS.bfs2
-
+               
 context Impl_Succ begin
 
     abbreviation "init_state_time == 3 + rbt_insert_logN 1 + rbt_insert_logN 1"
-    abbreviation "set_pick_time == 1"
 
 
-    abbreviation "bfs2 cf SS s t == Augmenting_Path_BFS.bfs2 cf
+lemma A: "Augmenting_Path_BFS set_pick_time map_lookup_time"
+  unfolding Augmenting_Path_BFS_def by simp
+    thm Augmenting_Path_BFS.bfs2_def
+
+
+
+
+definition init_state :: "nat \<Rightarrow> (bool \<times> (nat \<Rightarrow> nat option) \<times> nat set \<times> nat set \<times> nat) nrest" where
+  "init_state src = do {
+        m \<leftarrow> mop_map_empty (1::nat);
+        m \<leftarrow> mop_map_update (\<lambda>M. rbt_insert_logN (sizeM1' M)) m src src;
+        C \<leftarrow> mop_set_empty (1::nat);
+        C \<leftarrow> mop_set_insert (\<lambda>_. rbt_insert_logN (card C + 1)) src C;
+        N \<leftarrow> mop_set_empty (1::nat);
+        RETURNT (False, m, C, N, 0::nat)
+      }"
+
+    abbreviation "bfs2 cf SS IS s t == Augmenting_Path_BFS.bfs2 cf
                        set_insert_time map_dom_member_time  set_delete_time  map_update_time
-                      set_pick_time list_append_time map_lookup_time set_empty_time set_isempty_time init_state_time SS s t"
+                      set_pick_time list_append_time map_lookup_time set_empty_time set_isempty_time SS IS s t"
 
     definition op_bfs :: "'ga \<Rightarrow> node \<Rightarrow> node \<Rightarrow> path option nrest"
-      where [simp]: "op_bfs c s t \<equiv> bfs2 (absG c) (succ c) s t"
+      where [simp]: "op_bfs c s t \<equiv> bfs2 (absG c) (succ c) init_state s t"
   
    (* lemma pat_op_dfs[pat_rules]: 
       "bfs2$(absG$c)$(succ$c)$s$t \<equiv> UNPROTECT op_bfs$c$s$t" by simp 
@@ -31,31 +47,17 @@ context Impl_Succ begin
 
 
     type_synonym ibfs_state 
-      = "bool \<times> (node,node) i_map \<times> node set \<times> node set \<times> nat"
-
-    term Pre_BFS_Impl.init_state
-    thm Pre_BFS_Impl.init_state_def
+      = "bool \<times> (node \<rightharpoonup> node) \<times> node set \<times> node set \<times> nat"
+ 
 
 
     lemma P: "Pre_BFS_Impl set_pick_time" unfolding Pre_BFS_Impl_def by simp
-
-    definition "init_state = Pre_BFS_Impl.init_state init_state_time"
-
-definition init_state1 :: "nat \<Rightarrow> (bool \<times> (nat \<Rightarrow> nat option) \<times> nat set \<times> nat set \<times> nat) nrest" where
-  "init_state1 src = do {
-        m \<leftarrow> mop_map_empty 1;
-        m \<leftarrow> mop_map_update (\<lambda>M. rbt_insert_logN (sizeM1' M)) m src src;
-        C \<leftarrow> mop_set_empty 1;
-        C \<leftarrow> mop_set_insert (\<lambda>_. rbt_insert_logN (card C + 1)) src C;
-        N \<leftarrow> mop_set_empty 1;
-        RETURNT (False, m, C, N, 0)
-      }"
+ 
 
   
   
-  lemma "init_state1 src \<le> init_state src"
-    unfolding init_state1_def init_state_def 
-    unfolding Pre_BFS_Impl.init_state_def[OF P]
+  lemma "init_state src \<le> SPECT [ (False,[src\<mapsto>src],{src},{},0::nat) \<mapsto> init_state_time ]"
+    unfolding init_state_def   
     apply(rule T_specifies_I) unfolding mop_map_empty_def mop_map_update_def mop_set_empty_def
         mop_set_insert_def
       apply(vcg' \<open>clarsimp\<close>  ) by (simp add: sizeM1'_def) 
@@ -70,43 +72,151 @@ definition init_state1 :: "nat \<Rightarrow> (bool \<times> (nat \<Rightarrow> n
       notes [id_rules] = 
         itypeI[Pure.of src "TYPE(nat)"]
       shows "hn_refine (hn_val nat_rel src srci) 
-        (?c::?'c Heap) ?\<Gamma>' ?R (init_state1 src)"
+        (?c::?'c Heap) ?\<Gamma>' ?R (init_state src)"
       using [[id_debug, goals_limit = 1]]
-      unfolding init_state1_def   
+      unfolding init_state_def   
       apply sepref 
       done
       concrete_definition (in -) init_state_impl uses Impl_Succ.init_state_impl
 
       thm init_state_impl_def
-(*
-    lemmas [sepref_fr_rules] = init_state_impl.refine[OF this_loc,to_hfref]
-*)
 
+      lemmas [sepref_fr_rules] = init_state_impl.refine[OF this_loc,to_hfref]
+ 
+
+
+      thm Pre_BFS_Impl.pre_bfs2_def 
+lemma PP: "Pre_BFS_Impl set_pick_time" by(simp add: Pre_BFS_Impl_def)
+
+
+lemma (in -) hn_refine_Some[sepref_fr_rules]: " hn_refine (hn_val Id s' s)
+           (ureturn (Some s))
+       (hn_val Id s' s)
+       (pure Id) (RETURNT $ (Some $ s'))"
+  unfolding hn_refine_def apply (auto simp:   mult.assoc  execute_ureturn pure_def hn_ctxt_def)
+  by (auto simp: top_assn_rule zero_enat_def relH_def  elim: pureD )
+
+lemma (in -) hn_refine_Some_list[sepref_fr_rules]: " hn_refine (hn_ctxt (list_assn S) s' s)
+           (ureturn (Some s))
+       (hn_invalid (list_assn S) s' s)
+       ((option_assn (list_assn S))) (RETURNT $ (Some $ s'))" (*
+  unfolding hn_refine_def apply (auto simp:   mult.assoc  execute_ureturn pure_def hn_ctxt_def)
+  apply (auto simp: top_assn_rule zero_enat_def relH_def  elim: pureD )    
+  by (simp add: mod_star_trueI) *) sorry
+
+term mop_append
 
     schematic_goal bfs_impl:
       (*notes [sepref_opt_simps del] = imp_nfoldli_def 
           -- \<open>Prevent the foreach-loop to be unfolded to a fixed-point, 
               to produce more readable code for presentation purposes.\<close>*)
       notes [sepref_opt_simps] = heap_WHILET_def
-      fixes s t :: nat
+      fixes s t :: nat  
       notes [id_rules] = 
         itypeI[Pure.of s "TYPE(nat)"]
         itypeI[Pure.of t "TYPE(nat)"]
-        itypeI[Pure.of c "TYPE('ig)"]
+        itypeI[Pure.of c "TYPE('ig)"]  
         \<comment> \<open>Declare parameters to operation identification\<close>
-      shows "hn_refine (
+      shows
+"hn_refine (hn_ctxt isG c ci * hn_val nat_rel s si * hn_val nat_rel t ti) ?c ?\<Gamma>' ?R
+     (if s = t then RETURNT (Some [])
+      else (init_state s \<bind>
+            (\<lambda>sa. whileT (\<lambda>(f, PRED, C, N, d). f = False \<and> C \<noteq> {})
+                    (\<lambda>(f, PRED, C, N, d).
+                        ASSERT (C \<noteq> {}) \<bind>
+                        (\<lambda>_. mop_set_pick (Pre_BFS_Impl.setpickt set_pick_time) C \<bind>
+                              (\<lambda>v. mop_set_del (Pre_BFS_Impl.setdelt set_delete_time) C v \<bind>
+                                    (\<lambda>C. ASSERT (v \<in> Graph.V (absG c)) \<bind>
+                                          (\<lambda>_. succ c v \<bind>
+                                                (\<lambda>sl. RECT (\<lambda>D (l, s).
+case l of [] \<Rightarrow> RETURNT s
+| x # ls \<Rightarrow>
+    if case s of (f, PRED, N) \<Rightarrow> \<not> f
+    then (case s of
+          (f, PRED, N) \<Rightarrow>
+            mop_map_dom_member (\<lambda>_. map_dom_member_time) PRED x \<bind>
+            (\<lambda>b. if b then SPECT [(f, PRED, N) \<mapsto> enat 1]
+                  else mop_map_update (\<lambda>_. map_update_time) PRED x v \<bind>
+                       (\<lambda>PRED.
+                           ASSERT (x \<notin> N) \<bind>
+                           (\<lambda>_. mop_set_insert (\<lambda>_. set_insert_time) x N \<bind> (\<lambda>N. RETURNT (x = t, PRED, N)))))) \<bind>
+         (\<lambda>s. D (ls, s))
+    else RETURNT s)
+                                                        (sl, False, PRED, N) \<bind>
+                                                       (\<lambda>(f, PRED, N).
+                                                           if f then RETURNT (f, PRED, C, N, d + 1)
+                                                           else ASSERT
+ (case (f, PRED, C, N, d) of (f, PRED, C, N, d) \<Rightarrow> \<not> f \<and> nf_invar' (absG c) s t PRED C N d) \<bind>
+(\<lambda>_. mop_set_isempty (\<lambda>_. set_isempty_time) C \<bind>
+      (\<lambda>b. if b
+            then RETURNT N \<bind> (\<lambda>C. mop_set_empty set_empty_time \<bind> (\<lambda>N. RETURNT (d + 1) \<bind> (\<lambda>d. RETURNT (f, PRED, C, N, d))))
+            else RETURNT (f, PRED, C, N, d))))))))))
+                    sa \<bind>
+                   (\<lambda>(f, PRED, ttt, tt, d). if f then RETURNT (Some (d, PRED)) else RETURNT None))) \<bind>
+           (\<lambda>br.  case br of None \<Rightarrow> RETURNT None
+                  | Some (d, PRED) \<Rightarrow>  
+                      (whileT (\<lambda>(v, p). v \<noteq> s)
+                        (\<lambda>(v, p).
+                            ASSERT (v \<in> dom PRED) \<bind>
+                            (\<lambda>_. mop_map_lookup (\<lambda>_. map_lookup_time) PRED v \<bind> (\<lambda>u. 
+                                   mop_append (\<lambda>_. list_append_time) (u, v) p \<bind>  (\<lambda>p.  
+                                         RETURNT u \<bind> (\<lambda>v. RETURNT (v, p)))))
+              )  
+                        (t, ([]::((nat*nat) list))) \<bind>
+                       (\<lambda>(d, p). RETURNT p)) \<bind>
+                      (\<lambda>p. RETURNT (Some p))))   "
+
+      using [[id_debug, goals_limit = 2]]
+  apply sepref_dbg_preproc
+  apply sepref_dbg_cons_init
+  apply sepref_dbg_id_keep 
+     apply sepref_dbg_monadify
+     apply sepref_dbg_opt_init
+                                              
+  apply sepref_dbg_trans_step                 
+  apply sepref_dbg_trans_step                 
+  apply sepref_dbg_trans_step                 
+  apply sepref_dbg_trans_step                 
+  apply sepref_dbg_trans_step                 
+  apply sepref_dbg_trans_step                 
+  apply sepref_dbg_trans_step_keep oops                 
+  apply sepref_dbg_trans_step                 
+  apply sepref_dbg_trans_step                 
+  apply sepref_dbg_trans_step                 
+  apply sepref_dbg_trans_step                 
+  apply sepref_dbg_trans_step                 
+  apply sepref_dbg_trans_step                 
+  apply sepref_dbg_trans_step                 
+  apply sepref_dbg_trans_step                 
+  apply sepref_dbg_trans_step                 
+  apply sepref_dbg_trans_step                 
+  apply sepref_dbg_trans_step                 
+  apply sepref_dbg_trans_step                
+  apply sepref_dbg_trans_step_keep
+      oops
+  "hn_refine (
         hn_ctxt (isG) c ci 
       * hn_val nat_rel s si 
       * hn_val nat_rel t ti) (?c::?'c Heap) ?\<Gamma>' ?R (PR_CONST op_bfs c s t)"
       unfolding op_bfs_def PR_CONST_def
-      unfolding Graph.bfs2_def Graph.pre_bfs2_def 
-        Graph.inner_loop2_def Graph.extract_rpath_def
-      unfolding nres_monad_laws  
-      apply (rewrite in "nfoldli _ _ \<hole> _" fold_set_insert_dj)
-      apply (subst HOL_list.fold_custom_empty)+
-      apply (rewrite in "let N={} in _" ls.fold_custom_empty)
-      using [[id_debug, goals_limit = 1]]
-      apply sepref
+      unfolding Augmenting_Path_BFS.bfs2_def[OF A] unfolding Pre_BFS_Impl.pre_bfs2_def[OF PP]
+      unfolding Pre_BFS_Impl.inner_loop_def[OF PP]  unfolding  extract_rpath_def nfoldliIE_def nfoldli_def 
+      using [[id_debug, goals_limit = 2]]
+
+  apply sepref_dbg_preproc
+  apply sepref_dbg_cons_init
+  apply sepref_dbg_id_keep 
+     apply sepref_dbg_monadify
+
+     apply sepref_dbg_opt_init
+                                              
+  apply sepref_dbg_trans_step+ 
+
+  apply sepref_dbg_opt
+  apply sepref_dbg_cons_solve \<comment> \<open>Frame rule, recovering the invalidated list 
+    or pure elements, propagating recovery over the list structure\<close>
+  apply sepref_dbg_cons_solve \<comment> \<open>Trivial frame rule\<close>
+  apply sepref_dbg_constraints
       done
     
     concrete_definition (in -) bfs_impl uses Impl_Succ.bfs_impl
